<?xml version="1.0" encoding="UTF-8"?>
<rdf:RDF xmlns:rdf="http://www.w3.org/1999/02/22-rdf-syntax-ns#" xmlns:skos="http://www.w3.org/2004/02/skos/core#" xmlns:owl="http://www.w3.org/2002/07/owl#" xmlns:xsd="http://www.w3.org/2001/XMLSchema#" xmlns:swrl="http://www.w3.org/2003/11/swrl#" xmlns:swrlb="http://www.w3.org/2003/11/swrlb#" xmlns:rdfs="http://www.w3.org/2000/01/rdf-schema#" xml:base="https://ontology.swissartresearch.net/pwro/">
  <!--
						Extending the Art and Architectural Argumentation Ontology (AAAo), this project builds a set of classes and relations that enable the modelling of historical information pertaining to the exercise of power, the practice of religion, and the creation and maintenance of social relations through communicative acts.  Compatibility and Nomenclature  This unofficial extension of the CIDOC CRM is formulated in relation to:  CRM 7.1.3LRMoo 1.0CRMsci 2.0AAAo 2.0  The specification consists of a set of declarations for formalized classes and properties that extend the CIDOC CRM and the above official extensions.   Adopting the conventions of the CIDOC CRM each class and property have been given an identifier in addition to their names. The naming convention adopted for this extension is:  WE = classWP = property  The choice of these names was arbitrary, making a conceptual connection with the official CRM representation while clearly distinguishing the new classes and properties from those of either CRM base or its official extensions.  Namespace: https://ontology.swissartresearch.net/pwro/  Maintenance and Archiving  PWRo is an actively maintained ontology. It is our aim to develop publicly and participatively, learning from and engaging with the scholarly community that adopts it. Towards this end we maintain the ontology with the following processes and relative tools.  Ontology Development  We adopt the OntoMe tool developed by LARHRA to manage the ontology and produce editions. This ensures a consistent management of the ontology and provides a public space to engage in revisions.  The maintenace space for the ontology can be found here: https://ontome.net/project/208  Please note, at time of publishing, OntoME is not capable of producing complete, provenanced RDF serializations, so please only use the official RDF for this standard stored on our github. See below.   Issue Management and Revision Storage  We adopt github as a platform for inviting and managing issues related to the ontology as well as providing an active place to be able to access the latest edition of the ontology, its specification and relevant documentation.  The address for the github repository is: https://github.com/swiss-art-research-net/pwro   Acknowledgements  The initiative for creating, developing and maintaining this ontology is made possible by important on-going funding and institutional commitment, which is gratefully acknowledged here.  Funding Support:  The initial modelling around this extension have been supported by collaboration with the Releven: Re-evaluating the Eleventh Century and Globalise projects.  Institutional Support:    Swiss Art Research Infrastructure - University of Zurich  Takin.solutions  
						Exported from OntoME: Power, War, Religion and Relations Ontology ongoing
						Official URI : https://ontology.swissartresearch.net/pwro/
						-->
  <rdfs:Class rdf:about="https://ontology.swissartresearch.net/pwro/WE1_Exercise_of_Authority">
    <skos:notation rdf:datatype="http://www.w3.org/2001/XMLSchema#string">WE1</skos:notation>
    <rdfs:comment xml:lang="en" rdf:datatype="http://www.w3.org/2001/XMLSchema#string">This class comprises the activities involved in the exercise of power by a group or individual over some other persons and potentially some place. The exercise of authority is the active assertion of an individual or group's power over the related persons and/or place through physical and/or symbolic acts which are meant to and actually do maintain the authority of the individual or group exercising that power.
An instance of exercise of authority comes into existence through its assertion on the part of that power, which may bring about the authority of the individual or group asserting in question (e.g.: a declaration of authority by a party over some group or territory) or may represent a manifestation of the socially agreed upon application of the authority of an individual or group and their assumption of that authority (e.g.: appointment).
Instances of exercise of authority may cease to exist either through a counter action on the part of another (e.g.: seizing control of a ship), or through the socially agreed upon transfer of power (e.g.: end of term or removal from office). Moreover, the death of the individual or dissolution of the group exercising the authority in question may also brings about the end of existence of the exercise of authority.</rdfs:comment>
    <rdfs:label xml:lang="en">Exercise of Authority</rdfs:label>
    <rdfs:subClassOf rdf:resource="https://ontology.swissartresearch.net/aaao/ZE53_Symbolic_Act"/>
  </rdfs:Class>
  <rdfs:Class rdf:about="https://ontology.swissartresearch.net/pwro/WE2_Sovereignty">
    <skos:notation rdf:datatype="http://www.w3.org/2001/XMLSchema#string">WE2</skos:notation>
    <rdfs:comment xml:lang="en" rdf:datatype="http://www.w3.org/2001/XMLSchema#string">This class comprises the activities involved in the exercise of power by a ruling group or individual over a population and, typically, a territory. Sovereignty consists in the active assertion of the sovereign's power over the related population and territory through physical and/or symbolic acts which are meant to and actually do maintain the authority of that sovereign.
An instance of sovereignty may come into existence either through its assertion on the part of the sovereign, which may bring about the rule of the sovereign (e.g.: a revolution, coup d'etat) or may come about constitutionally through the application of pre-agreed terms of the declaration of a new sovereign and their assumption of sovereignty (e.g.: coronation procedures).
Instances of sovereignty may cease to exist either through a counter action that successfully challenges that sovereignty (e.g., a popular revolution), through the dissolution of general social order, or constitutionally through pre-agreed forms of the transfer of power (e.g., direct descent). Moreover, the death or dissolution of the individual or group exercising sovereignty may also bring about the end to its existence.</rdfs:comment>
    <rdfs:label xml:lang="en">Sovereignty</rdfs:label>
    <rdfs:subClassOf rdf:resource="https://ontology.swissartresearch.net/pwro/WE1_Exercise_of_Authority"/>
  </rdfs:Class>
  <rdfs:Class rdf:about="https://ontology.swissartresearch.net/pwro/WE3_Embodied_Actor">
    <skos:notation rdf:datatype="http://www.w3.org/2001/XMLSchema#string">WE3</skos:notation>
    <rdfs:comment xml:lang="en" rdf:datatype="http://www.w3.org/2001/XMLSchema#string">This class comprises persons be they animal or more specifically human animals, individually or collectively in embodied form. The substance of embodied actor is physical persons.
Instances of embodied actor come to be when the individual be it singular or plural is fully manifest in reality and agentially capable (in the broad sense of the term). Instances of embodied actor cease to exist when, if individual, they are materially and/or agentially defunct, having undergone physical or noetic disintegration, and when, if grouped, they are substantially dispersed after they have come together for a particular purpose.</rdfs:comment>
    <rdfs:label xml:lang="en">Embodied Actor</rdfs:label>
    <rdfs:subClassOf rdf:resource="http://www.cidoc-crm.org/cidoc-crm/E20_Biological_Object"/>
    <rdfs:subClassOf rdf:resource="http://www.cidoc-crm.org/cidoc-crm/E39_Actor"/>
  </rdfs:Class>
  <rdfs:Class rdf:about="https://ontology.swissartresearch.net/pwro/WE4_Manifest_Group">
    <skos:notation rdf:datatype="http://www.w3.org/2001/XMLSchema#string">WE4</skos:notation>
    <rdfs:comment xml:lang="en" rdf:datatype="http://www.w3.org/2001/XMLSchema#string">This class comprises a defined set of persons who are able to act together as a single collective in intentional action and who are moreover gathered together physically to bring about this end. The substance of manifest groups is physical persons qua embodied actor.
Instances of manifest group come into existence when an intentional group maintains a continuous co-presence in spacetime. Instances of manifest group cease to exist when this co-presence ends.
Examples of manifest group include the players playing in a particular football match, the soldiers deployed in a battalion for a particular battle, a herd of sheep.</rdfs:comment>
    <rdfs:label xml:lang="en">Manifest Group</rdfs:label>
    <rdfs:subClassOf rdf:resource="https://ontology.swissartresearch.net/pwro/WE3_Embodied_Actor"/>
    <rdfs:subClassOf rdf:resource="http://www.cidoc-crm.org/cidoc-crm/E74_Group"/>
  </rdfs:Class>
  <rdfs:Class rdf:about="https://ontology.swissartresearch.net/pwro/WE5_Animal">
    <skos:notation rdf:datatype="http://www.w3.org/2001/XMLSchema#string">WE5</skos:notation>
    <rdfs:comment xml:lang="en" rdf:datatype="http://www.w3.org/2001/XMLSchema#string">Instances of this class are living organisms that move and react to the environment around themselves and are endowed with some level of sentience.</rdfs:comment>
    <rdfs:label xml:lang="en">Animal</rdfs:label>
    <rdfs:subClassOf rdf:resource="https://ontology.swissartresearch.net/pwro/WE3_Embodied_Actor"/>
  </rdfs:Class>
  <rdfs:Class rdf:about="https://ontology.swissartresearch.net/pwro/WE6_Attack">
    <skos:notation rdf:datatype="http://www.w3.org/2001/XMLSchema#string">WE6</skos:notation>
    <rdfs:comment xml:lang="en" rdf:datatype="http://www.w3.org/2001/XMLSchema#string">This class comprises instances of aggressive physical action by one party towards another in which the instigator intends to cause damage to the target.</rdfs:comment>
    <rdfs:label xml:lang="en">Attack</rdfs:label>
    <rdfs:subClassOf rdf:resource="https://ontology.swissartresearch.net/aaao/ZE53_Symbolic_Act"/>
  </rdfs:Class>
  <rdfs:Class rdf:about="https://ontology.swissartresearch.net/pwro/WE7_Voyage">
    <skos:notation rdf:datatype="http://www.w3.org/2001/XMLSchema#string">WE7</skos:notation>
    <rdfs:comment xml:lang="en" rdf:datatype="http://www.w3.org/2001/XMLSchema#string">This class comprises events in which physical objects are moved from one place to another and wherein either the main or one of the main objects being moved is the person or persons undertaking the voyage. The substance of this class is that of an intentional event.
Instance of voyage come into existence when the intention to voyage is declared and the associated preparative actions are begun with the intention of actually leaving. An instance of voyage may come to an end when it reaches its intended destination. It may also end if the intention to voyage is abandoned or the means by which to achieve it are no longer available.</rdfs:comment>
    <rdfs:label xml:lang="en">Voyage</rdfs:label>
    <rdfs:subClassOf rdf:resource="https://ontology.swissartresearch.net/pwro/WE12_Sending"/>
  </rdfs:Class>
  <rdfs:Class rdf:about="https://ontology.swissartresearch.net/pwro/WE8_Intentional_Destruction">
    <skos:notation rdf:datatype="http://www.w3.org/2001/XMLSchema#string">WE8</skos:notation>
    <rdfs:comment xml:lang="en" rdf:datatype="http://www.w3.org/2001/XMLSchema#string">This class comprises events which are deliberately undertaken to cause the destruction of some physical thing and which succeed in that effort. The substance of this class is intentional activity with intent to destroy.
Instances of this class come into existence when an actor begins an action that is intended to and capable of bringing about the end of existence of a physical object through an injurious action. Instances of this class cease to be when the aim of destroying the object is achieved and the object is destroyed.</rdfs:comment>
    <rdfs:label xml:lang="en">Intentional Destruction</rdfs:label>
    <rdfs:subClassOf rdf:resource="https://ontology.swissartresearch.net/pwro/WE9_Destructive_Physical_Modification"/>
    <rdfs:subClassOf rdf:resource="http://www.cidoc-crm.org/cidoc-crm/E6_Destruction"/>
  </rdfs:Class>
  <rdfs:Class rdf:about="https://ontology.swissartresearch.net/pwro/WE9_Destructive_Physical_Modification">
    <skos:notation rdf:datatype="http://www.w3.org/2001/XMLSchema#string">WE9</skos:notation>
    <rdfs:comment xml:lang="en" rdf:datatype="http://www.w3.org/2001/XMLSchema#string">This class comprises instances of intentional action by actors that are undertaken to physically bring about constitutional degradation and harm to physical things
An instance of this class comes into existence when an actor undertakes to bring about damage to a physical thing with appropriate equipment and planning according to the context and intended object of damage to bring about such harm. Instances of this class come to a halt when the intended damage has been achieved or if the initiated action is given up part way or through lack of will or means to finish the action.</rdfs:comment>
    <rdfs:label xml:lang="en">Destructive Physical Modification</rdfs:label>
    <rdfs:subClassOf rdf:resource="http://www.cidoc-crm.org/cidoc-crm/E7_Activity"/>
  </rdfs:Class>
  <rdfs:Class rdf:about="https://ontology.swissartresearch.net/pwro/WE10_Ameliorative_Physical_Modification">
    <skos:notation rdf:datatype="http://www.w3.org/2001/XMLSchema#string">WE10</skos:notation>
    <rdfs:comment xml:lang="en" rdf:datatype="http://www.w3.org/2001/XMLSchema#string">This class comprises instances of intentional action by actors that are undertaken to physically bring about constitutional improvement and benefit to E18 Physical Things.
An instance of this class comes into existence when an actor undertakes to bring about benefit to a physical thing with appropriate equipment and planning according to the context and intended object of amelioration to bring about such benefit. Instances of this class come to a halt when the intended benefit has been achieved or if the initiated action is given up part way or through lack of will or means to finish the action.</rdfs:comment>
    <rdfs:label xml:lang="en">Ameliorative Physical Modification</rdfs:label>
    <rdfs:subClassOf rdf:resource="http://www.cidoc-crm.org/cidoc-crm/E7_Activity"/>
  </rdfs:Class>
  <rdfs:Class rdf:about="https://ontology.swissartresearch.net/pwro/WE11_Correspondence_Event">
    <skos:notation rdf:datatype="http://www.w3.org/2001/XMLSchema#string">WE11</skos:notation>
    <rdfs:comment xml:lang="en" rdf:datatype="http://www.w3.org/2001/XMLSchema#string">Instances of this class represent communicative acts in which an actor addresses a message to another person or set of persons. </rdfs:comment>
    <rdfs:label xml:lang="en">Correspondence Event</rdfs:label>
    <rdfs:subClassOf rdf:resource="http://iflastandards.info/ns/lrm/lrmoo/F28"/>
  </rdfs:Class>
  <rdfs:Class rdf:about="https://ontology.swissartresearch.net/pwro/WE12_Sending">
    <skos:notation rdf:datatype="http://www.w3.org/2001/XMLSchema#string">WE12</skos:notation>
    <rdfs:comment xml:lang="en" rdf:datatype="http://www.w3.org/2001/XMLSchema#string">This class comprises events in which physical objects are moved from one place to another and wherein the sending person is not also the object of the event. The substance of this class is that of an intentional activity. Particularly, it is typical to know the declared origin and destination of an instance of sending but not necessarily its eventual outcome.
An instance of sending comes into existence when the requisite actions are undertaken to initiate the dispatch of a physical object from one place to another are put it place and the sending made possible. An instance of sending may come to an end when the object sent has reached its intended destination. It may also end if the intention to send is abandoned or the means by which to achieve it are no longer available.</rdfs:comment>
    <rdfs:label xml:lang="en">Sending</rdfs:label>
    <rdfs:subClassOf rdf:resource="http://www.cidoc-crm.org/cidoc-crm/E9_Move"/>
  </rdfs:Class>
  <rdfs:Class rdf:about="https://ontology.swissartresearch.net/pwro/WE13_Visit">
    <skos:notation rdf:datatype="http://www.w3.org/2001/XMLSchema#string">WE13</skos:notation>
    <rdfs:comment xml:lang="en" rdf:datatype="http://www.w3.org/2001/XMLSchema#string">Instances of this class involve the intentional activity of actors to spend time in a geographic location for the sake of exploring and generally 'being' at that place for a period of time. Instances of visit entail an intentional relation to the place visited by the intending actor, engaging in interaction with and observation of the place that they visit and the various things to be met in that space.
Instances of visit begin with the arrival of the visiting actor within the place to be visited. Instances of visit end when the visiting actor leaves the place visited. Instances of visit may further end if the actor gives up the intention or loses the means by which to continue the visit or themselves expire.</rdfs:comment>
    <rdfs:label xml:lang="en">Visit</rdfs:label>
    <rdfs:subClassOf rdf:resource="http://www.cidoc-crm.org/cidoc-crm/E7_Activity"/>
  </rdfs:Class>
  <rdfs:Class rdf:about="https://ontology.swissartresearch.net/pwro/WE14_Dwelling">
    <skos:notation rdf:datatype="http://www.w3.org/2001/XMLSchema#string">WE14</skos:notation>
    <rdfs:comment xml:lang="en" rdf:datatype="http://www.w3.org/2001/XMLSchema#string">Instances of this class involve the intentional activity of actors to spend time in a geographic location in a capacity as inhabitant. Instances of dwelling entail an intentional relation to the place dwelt in by the intending actor, engaging in interaction with and observation of the place dwelt in and the various things to be met in that space in a manner building up a longer term relation to and reliance on the latter.
Instances of dwelling begin with the settling in of the dwelling actor within the place to be dwelt in. Instances of dwelling end when the dwelling actor permanently leaves the place dwelt in, typically to establish dwelling in another place. Instances of dwelling may further end if the actor is forced against their will or lose the means by which to continue the dwelling in that place or when they themselves expire.</rdfs:comment>
    <rdfs:label xml:lang="en">Dwelling</rdfs:label>
    <rdfs:subClassOf rdf:resource="http://www.cidoc-crm.org/cidoc-crm/E7_Activity"/>
  </rdfs:Class>
  <rdfs:Class rdf:about="https://ontology.swissartresearch.net/pwro/WE15_Act_of_Authority">
    <skos:notation rdf:datatype="http://www.w3.org/2001/XMLSchema#string">WE15</skos:notation>
    <rdfs:comment xml:lang="en" rdf:datatype="http://www.w3.org/2001/XMLSchema#string">This class comprises instances of commands, orders, requests, etc., undertaken on the basis of one's authority, which typically aim to trigger a subsequent event, itself carried out by those who recognize the authority status of the actor. An instance of act of authority is conducted within a social-cultural framework and makes use of the codes and symbols of that framework to initiate an event or a sequence of events aimed at realising some desired outcome.
Instances of act of authority begin when an E39 Actor, endowed with the appropriate authority, has another E39 Actor undertake an action by invoking an existing code or procedure to trigger the desired outcome. This need not, however, refer to an explicit or formal code or procedure.</rdfs:comment>
    <rdfs:label xml:lang="en">Act of Authority</rdfs:label>
    <rdfs:subClassOf rdf:resource="https://ontology.swissartresearch.net/aaao/ZE53_Symbolic_Act"/>
  </rdfs:Class>
  <rdf:Property rdf:about="https://ontology.swissartresearch.net/pwro/WP1_had_geographic_scope">
    <rdfs:range rdf:resource="http://www.cidoc-crm.org/cidoc-crm/E53_Place"/>
    <rdfs:comment xml:lang="en">This property relates an instance of exercise of authority to the location over which it projects this authority.</rdfs:comment>
    <rdfs:label xml:lang="en">had geographic scope</rdfs:label>
    <skos:notation rdf:datatype="http://www.w3.org/2001/XMLSchema#string">WP1</skos:notation>
    <rdfs:domain rdf:resource="https://ontology.swissartresearch.net/pwro/WE1_Exercise_of_Authority"/>
  </rdf:Property>
  <rdf:Property rdf:about="https://ontology.swissartresearch.net/pwro/WP2_had_authority_over">
    <rdfs:range rdf:resource="https://ontology.swissartresearch.net/aaao/ZE36_Persons"/>
    <rdfs:comment xml:lang="en">This property connects an instance of exercise of authority to the persons individually or collectively over whom it exercised authority.</rdfs:comment>
    <rdfs:label xml:lang="en">had authority over</rdfs:label>
    <skos:notation rdf:datatype="http://www.w3.org/2001/XMLSchema#string">WP2</skos:notation>
    <rdfs:domain rdf:resource="https://ontology.swissartresearch.net/pwro/WE1_Exercise_of_Authority"/>
    <rdfs:subPropertyOf rdf:resource="http://www.cidoc-crm.org/cidoc-crm/P11_had_participant"/>
  </rdf:Property>
  <rdf:Property rdf:about="https://ontology.swissartresearch.net/pwro/WP3_had_sovereign">
    <rdfs:range rdf:resource="http://www.cidoc-crm.org/cidoc-crm/E39_Actor"/>
    <rdfs:comment xml:lang="en">This property relates an instance of sovereignty to an actor, individual or group, who wielded that sovereignty.</rdfs:comment>
    <rdfs:label xml:lang="en">had sovereign</rdfs:label>
    <skos:notation rdf:datatype="http://www.w3.org/2001/XMLSchema#string">WP3</skos:notation>
    <rdfs:domain rdf:resource="https://ontology.swissartresearch.net/pwro/WE2_Sovereignty"/>
    <rdfs:subPropertyOf rdf:resource="http://www.cidoc-crm.org/cidoc-crm/P14_carried_out_by"/>
  </rdf:Property>
  <rdf:Property rdf:about="https://ontology.swissartresearch.net/pwro/WP4_had_subject_population">
    <rdfs:range rdf:resource="https://ontology.swissartresearch.net/aaao/ZE37_Population"/>
    <rdfs:comment xml:lang="en">This property relates an instance of sovereignty to a population over which it wielded this sovereignty.</rdfs:comment>
    <rdfs:label xml:lang="en">had subject population</rdfs:label>
    <skos:notation rdf:datatype="http://www.w3.org/2001/XMLSchema#string">WP4</skos:notation>
    <rdfs:domain rdf:resource="https://ontology.swissartresearch.net/pwro/WE2_Sovereignty"/>
    <rdfs:subPropertyOf rdf:resource="https://ontology.swissartresearch.net/pwro/WP2_had_authority_over"/>
  </rdf:Property>
  <rdf:Property rdf:about="https://ontology.swissartresearch.net/pwro/WP5_was_manifestation_of">
    <rdfs:range rdf:resource="http://www.cidoc-crm.org/cidoc-crm/E74_Group"/>
    <rdfs:comment xml:lang="en">This property relates an instance of manifest group as a realized collection of real individuals formed together in a coherent space time volume at some time to the abstract group with which they are otherwise identified.</rdfs:comment>
    <rdfs:label xml:lang="en">was manifestation of</rdfs:label>
    <skos:notation rdf:datatype="http://www.w3.org/2001/XMLSchema#string">WP5</skos:notation>
    <rdfs:domain rdf:resource="https://ontology.swissartresearch.net/pwro/WE4_Manifest_Group"/>
  </rdf:Property>
  <rdf:Property rdf:about="https://ontology.swissartresearch.net/pwro/WP6_had_intended_target">
    <rdfs:range rdf:resource="http://www.cidoc-crm.org/cidoc-crm/E18_Physical_Thing"/>
    <rdfs:comment xml:lang="en">This property relates an instance of attack to the intended target of that attack.</rdfs:comment>
    <rdfs:label xml:lang="en">had intended target</rdfs:label>
    <skos:notation rdf:datatype="http://www.w3.org/2001/XMLSchema#string">WP6</skos:notation>
    <rdfs:domain rdf:resource="https://ontology.swissartresearch.net/pwro/WE6_Attack"/>
  </rdf:Property>
  <rdf:Property rdf:about="https://ontology.swissartresearch.net/pwro/WP7_was_undertaken_by">
    <rdfs:range rdf:resource="https://ontology.swissartresearch.net/pwro/WE3_Embodied_Actor"/>
    <rdfs:comment xml:lang="en">This property links an instance of voyage to an instance of embodied actor that undertook that voyage. The related embodied actor is both the agent carrying out the voyage and the object moved. </rdfs:comment>
    <rdfs:label xml:lang="en">was undertaken by</rdfs:label>
    <skos:notation rdf:datatype="http://www.w3.org/2001/XMLSchema#string">WP7</skos:notation>
    <rdfs:domain rdf:resource="https://ontology.swissartresearch.net/pwro/WE7_Voyage"/>
    <rdfs:subPropertyOf rdf:resource="http://www.cidoc-crm.org/cidoc-crm/P14_carried_out_by"/>
    <rdfs:subPropertyOf rdf:resource="http://www.cidoc-crm.org/cidoc-crm/P25_moved"/>
  </rdf:Property>
  <rdf:Property rdf:about="https://ontology.swissartresearch.net/pwro/WP8_had_declared_intermediary_place">
    <rdfs:range rdf:resource="http://www.cidoc-crm.org/cidoc-crm/E53_Place"/>
    <rdfs:comment xml:lang="en">This property links an instance of voyage to an instance of place that the voyage was intended to pass through in the context of the voyage. The connection created between the voyage and the place is one of intention. Whether a place was actually passed through can only be determined by further documentation which would motivate the documentation of a visit or stop at the intended intermediary place as part of the overall instance of voyage.</rdfs:comment>
    <rdfs:label xml:lang="en">had declared intermediary place</rdfs:label>
    <skos:notation rdf:datatype="http://www.w3.org/2001/XMLSchema#string">WP8</skos:notation>
    <rdfs:domain rdf:resource="https://ontology.swissartresearch.net/pwro/WE7_Voyage"/>
  </rdf:Property>
  <rdf:Property rdf:about="https://ontology.swissartresearch.net/pwro/WP9_had_declared_destination">
    <rdfs:range rdf:resource="http://www.cidoc-crm.org/cidoc-crm/E53_Place"/>
    <rdfs:comment xml:lang="en">This property links an instance of sending (and its subclasses) with a place of intended destination for the sending of the object. This property links the act of sending with the referenced place through intention, enabling the representation of the intended final arrival spot of the sent object. In documentation, an intended destination may be known rather than an actual destination of arrival for the sent object, or the intended destination and the final destination differ. This property allows the description of this nuance. The property crm:P26_moved_to should be used to document an actual move. For more complex, multi part actions of sending, an event forming part of the overall sending may document the final arrival place of the object (be that at its intended or another location).</rdfs:comment>
    <rdfs:label xml:lang="en">had declared destination</rdfs:label>
    <skos:notation rdf:datatype="http://www.w3.org/2001/XMLSchema#string">WP9</skos:notation>
    <rdfs:domain rdf:resource="https://ontology.swissartresearch.net/pwro/WE12_Sending"/>
  </rdf:Property>
  <rdf:Property rdf:about="https://ontology.swissartresearch.net/pwro/WP10_diminished">
    <rdfs:range rdf:resource="http://www.cidoc-crm.org/cidoc-crm/E18_Physical_Thing"/>
    <rdfs:comment xml:lang="en">This property links an instance of destructive physical modification with an instance of physical thing that was diminished through this activity. This property enables the documentation that an instance of destructive physical modification successfully resulted in the reduction of the physical integrity of the physical thing targeted. It does not enable the quantification of this diminishing effect.</rdfs:comment>
    <rdfs:label xml:lang="en">diminished</rdfs:label>
    <skos:notation rdf:datatype="http://www.w3.org/2001/XMLSchema#string">WP10</skos:notation>
    <rdfs:domain rdf:resource="https://ontology.swissartresearch.net/pwro/WE9_Destructive_Physical_Modification"/>
    <rdfs:subPropertyOf rdf:resource="http://www.cidoc-crm.org/cidoc-crm/P12_occurred_in_the_presence_of"/>
  </rdf:Property>
  <rdf:Property rdf:about="https://ontology.swissartresearch.net/pwro/WP11_ameliorated">
    <rdfs:range rdf:resource="http://www.cidoc-crm.org/cidoc-crm/E18_Physical_Thing"/>
    <rdfs:comment xml:lang="en">This property links an instance of ameliorative physical modification with an instance of physical thing that was ameliorated through this activity. This property enables the documentation that an instance of ameliorative physical modification successfully resulted in the improvement of the physical integrity of the physical thing targeted. It does not enable the quantification of this salutary effect.</rdfs:comment>
    <rdfs:label xml:lang="en">ameliorated</rdfs:label>
    <skos:notation rdf:datatype="http://www.w3.org/2001/XMLSchema#string">WP11</skos:notation>
    <rdfs:domain rdf:resource="https://ontology.swissartresearch.net/pwro/WE10_Ameliorative_Physical_Modification"/>
    <rdfs:subPropertyOf rdf:resource="http://www.cidoc-crm.org/cidoc-crm/P12_occurred_in_the_presence_of"/>
  </rdf:Property>
  <rdf:Property rdf:about="https://ontology.swissartresearch.net/pwro/WP12_had_addressee">
    <rdfs:range rdf:resource="https://ontology.swissartresearch.net/aaao/ZE36_Persons"/>
    <rdfs:comment xml:lang="en">This property links an instance of correspondence event to an instance of  persons to whom it is addressed. This property enables the documentation in a chain of communication of the intended receiver of a particular act of communicating a message.</rdfs:comment>
    <rdfs:label xml:lang="en">had addressee</rdfs:label>
    <skos:notation rdf:datatype="http://www.w3.org/2001/XMLSchema#string">WP12</skos:notation>
    <rdfs:domain rdf:resource="https://ontology.swissartresearch.net/pwro/WE11_Correspondence_Event"/>
  </rdf:Property>
  <rdf:Property rdf:about="https://ontology.swissartresearch.net/pwro/WP13_had_declared_origin">
    <rdfs:range rdf:resource="http://www.cidoc-crm.org/cidoc-crm/E53_Place"/>
    <rdfs:comment xml:lang="en">This property links an instance of sending (and its subclasses) with a place of intended origin for the sending of the object. This property links the act of sending with the referenced place through intention, enabling the representation of the intended originating location of the sending activity. In documentation, an intended origin destination may be known in distinction to the actual origin destination of the sending, and indeed the intended origin location and the final origin location may actually differ. This property allows the description of this nuance. The property crm:P27_moved_from should be used to document an actual origin location. For more complex, multi part actions of sending, an event forming part of the overall sending may document the final origin place of the sending (be that at its intended or another location).</rdfs:comment>
    <rdfs:label xml:lang="en">had declared origin</rdfs:label>
    <skos:notation rdf:datatype="http://www.w3.org/2001/XMLSchema#string">WP13</skos:notation>
    <rdfs:domain rdf:resource="https://ontology.swissartresearch.net/pwro/WE12_Sending"/>
  </rdf:Property>
  <rdf:Property rdf:about="https://ontology.swissartresearch.net/pwro/WP14_visited">
    <rdfs:range rdf:resource="http://www.cidoc-crm.org/cidoc-crm/E53_Place"/>
    <rdfs:comment xml:lang="en">This property enables the documentation of the relation of an instance of visit event to the place visited. The relation holding between the visit event and the place differs from the typical documentation of the place at which an event occurs. The documented of the visit relation indicates the intentional activity of the actors involved to interact with and observe the place visited and the objects / events occurring within this place frame.
 </rdfs:comment>
    <rdfs:label xml:lang="en">visited</rdfs:label>
    <skos:notation rdf:datatype="http://www.w3.org/2001/XMLSchema#string">WP14</skos:notation>
    <rdfs:domain rdf:resource="https://ontology.swissartresearch.net/pwro/WE13_Visit"/>
    <rdfs:subPropertyOf rdf:resource="http://www.cidoc-crm.org/cidoc-crm/P7_took_place_at"/>
  </rdf:Property>
  <rdf:Property rdf:about="https://ontology.swissartresearch.net/pwro/WP15_dwelt_in">
    <rdfs:range rdf:resource="http://www.cidoc-crm.org/cidoc-crm/E53_Place"/>
    <rdfs:comment xml:lang="en">This property enables the documentation of the relation of an instance of dwelling event to the place dwelt in. The relation holding between the dwelling event and the place differs from the typical documentation of the place at which an event occurs. The documentation of the dwelling relation indicates the intentional activity of the actors involved to take up phenomenal residence and interact with the place dwelt in and the objects / events occurring therein as part of their everyday life and life activity.</rdfs:comment>
    <rdfs:label xml:lang="en">dwelt in</rdfs:label>
    <skos:notation rdf:datatype="http://www.w3.org/2001/XMLSchema#string">WP15</skos:notation>
    <rdfs:domain rdf:resource="https://ontology.swissartresearch.net/pwro/WE14_Dwelling"/>
    <rdfs:subPropertyOf rdf:resource="http://www.cidoc-crm.org/cidoc-crm/P7_took_place_at"/>
  </rdf:Property>
  <rdf:Property rdf:about="https://ontology.swissartresearch.net/pwro/WP16_had_combatant">
    <rdfs:range rdf:resource="https://ontology.swissartresearch.net/pwro/WE3_Embodied_Actor"/>
    <rdfs:comment xml:lang="en">This property links an event of attack to instances of embodied actor who actively took part in the physical act of attacking.</rdfs:comment>
    <rdfs:label xml:lang="en">had combatant</rdfs:label>
    <skos:notation rdf:datatype="http://www.w3.org/2001/XMLSchema#string">WP16</skos:notation>
    <rdfs:domain rdf:resource="https://ontology.swissartresearch.net/pwro/WE6_Attack"/>
    <rdfs:subPropertyOf rdf:resource="http://www.cidoc-crm.org/cidoc-crm/P12_occurred_in_the_presence_of"/>
    <rdfs:subPropertyOf rdf:resource="http://www.cidoc-crm.org/cidoc-crm/P14_carried_out_by"/>
  </rdf:Property>
  <rdf:Property rdf:about="https://ontology.swissartresearch.net/pwro/WP1i_was_geographic_scope_of">
    <rdfs:domain rdf:resource="http://www.cidoc-crm.org/cidoc-crm/E53_Place"/>
    <rdfs:comment xml:lang="en">This property is the inverse of the forward property described in the scope note that follows. This property relates an instance of exercise of authority to the location over which it projects this authority.</rdfs:comment>
    <rdfs:label xml:lang="en">was geographic scope of</rdfs:label>
    <skos:notation rdf:datatype="http://www.w3.org/2001/XMLSchema#string">WP1i</skos:notation>
    <rdfs:range rdf:resource="https://ontology.swissartresearch.net/pwro/WE1_Exercise_of_Authority"/>
  </rdf:Property>
  <rdf:Property rdf:about="https://ontology.swissartresearch.net/pwro/WP2i_was_subject_to_authority_of">
    <rdfs:domain rdf:resource="https://ontology.swissartresearch.net/aaao/ZE36_Persons"/>
    <rdfs:comment xml:lang="en">This property is the inverse of the forward property described in the scope note that follows. This property connects an instance of exercise of authority to the persons individually or collectively over whom it exercised authority.</rdfs:comment>
    <rdfs:label xml:lang="en">was subject to authority of</rdfs:label>
    <skos:notation rdf:datatype="http://www.w3.org/2001/XMLSchema#string">WP2i</skos:notation>
    <rdfs:range rdf:resource="https://ontology.swissartresearch.net/pwro/WE1_Exercise_of_Authority"/>
    <rdfs:subPropertyOf rdf:resource="http://www.cidoc-crm.org/cidoc-crm/P11i_participated_in"/>
  </rdf:Property>
  <rdf:Property rdf:about="https://ontology.swissartresearch.net/pwro/WP3i_exercised_authority_of">
    <rdfs:domain rdf:resource="http://www.cidoc-crm.org/cidoc-crm/E39_Actor"/>
    <rdfs:comment xml:lang="en">This property is the inverse of the forward property described in the scope note that follows. This property relates an instance of sovereignty to an actor, individual or group, who wielded that sovereignty.</rdfs:comment>
    <rdfs:label xml:lang="en">exercised authority of</rdfs:label>
    <skos:notation rdf:datatype="http://www.w3.org/2001/XMLSchema#string">WP3i</skos:notation>
    <rdfs:range rdf:resource="https://ontology.swissartresearch.net/pwro/WE2_Sovereignty"/>
    <rdfs:subPropertyOf rdf:resource="http://www.cidoc-crm.org/cidoc-crm/P14i_performed"/>
  </rdf:Property>
  <rdf:Property rdf:about="https://ontology.swissartresearch.net/pwro/WP4i_was_subject_population_of">
    <rdfs:domain rdf:resource="https://ontology.swissartresearch.net/aaao/ZE37_Population"/>
    <rdfs:comment xml:lang="en">This property is the inverse of the forward property described in the scope note that follows. This property relates an instance of sovereignty to a population over which it wielded this sovereignty.</rdfs:comment>
    <rdfs:label xml:lang="en">was subject population of</rdfs:label>
    <skos:notation rdf:datatype="http://www.w3.org/2001/XMLSchema#string">WP4i</skos:notation>
    <rdfs:range rdf:resource="https://ontology.swissartresearch.net/pwro/WE2_Sovereignty"/>
    <rdfs:subPropertyOf rdf:resource="https://ontology.swissartresearch.net/pwro/WP2i_was_subject_to_authority_of"/>
  </rdf:Property>
  <rdf:Property rdf:about="https://ontology.swissartresearch.net/pwro/WP5i_manifested_in">
    <rdfs:domain rdf:resource="http://www.cidoc-crm.org/cidoc-crm/E74_Group"/>
    <rdfs:comment xml:lang="en">This property is the inverse of the forward property described in the scope note that follows. This property relates an instance of manifest group as a realized collection of real individuals formed together in a coherent space time volume at some time to the abstract group with which they are otherwise identified.</rdfs:comment>
    <rdfs:label xml:lang="en">manifested in</rdfs:label>
    <skos:notation rdf:datatype="http://www.w3.org/2001/XMLSchema#string">WP5i</skos:notation>
    <rdfs:range rdf:resource="https://ontology.swissartresearch.net/pwro/WE4_Manifest_Group"/>
  </rdf:Property>
  <rdf:Property rdf:about="https://ontology.swissartresearch.net/pwro/WP6i_was_intended_target_of">
    <rdfs:domain rdf:resource="http://www.cidoc-crm.org/cidoc-crm/E18_Physical_Thing"/>
    <rdfs:comment xml:lang="en">This property is the inverse of the forward property described in the scope note that follows. This property relates an instance of attack to the intended target of that attack.</rdfs:comment>
    <rdfs:label xml:lang="en">was intended target of</rdfs:label>
    <skos:notation rdf:datatype="http://www.w3.org/2001/XMLSchema#string">WP6i</skos:notation>
    <rdfs:range rdf:resource="https://ontology.swissartresearch.net/pwro/WE6_Attack"/>
  </rdf:Property>
  <rdf:Property rdf:about="https://ontology.swissartresearch.net/pwro/WP7i_undertook">
    <rdfs:domain rdf:resource="https://ontology.swissartresearch.net/pwro/WE3_Embodied_Actor"/>
    <rdfs:comment xml:lang="en">This property is the inverse of the forward property described in the scope note that follows. This property links an instance of voyage to an instance of embodied actor that undertook that voyage. The related embodied actor is both the agent carrying out the voyage and the object moved. </rdfs:comment>
    <rdfs:label xml:lang="en">undertook</rdfs:label>
    <skos:notation rdf:datatype="http://www.w3.org/2001/XMLSchema#string">WP7i</skos:notation>
    <rdfs:range rdf:resource="https://ontology.swissartresearch.net/pwro/WE7_Voyage"/>
    <rdfs:subPropertyOf rdf:resource="http://www.cidoc-crm.org/cidoc-crm/P14i_performed"/>
    <rdfs:subPropertyOf rdf:resource="http://www.cidoc-crm.org/cidoc-crm/P25i_moved_by"/>
  </rdf:Property>
  <rdf:Property rdf:about="https://ontology.swissartresearch.net/pwro/WP8i_was_declared_intermediary_place_of">
    <rdfs:domain rdf:resource="http://www.cidoc-crm.org/cidoc-crm/E53_Place"/>
    <rdfs:comment xml:lang="en">This property is the inverse of the forward property described in the scope note that follows. This property links an instance of voyage to an instance of place that the voyage was intended to pass through in the context of the voyage. The connection created between the voyage and the place is one of intention. Whether a place was actually passed through can only be determined by further documentation which would motivate the documentation of a visit or stop at the intended intermediary place as part of the overall instance of voyage.</rdfs:comment>
    <rdfs:label xml:lang="en">was declared intermediary place of</rdfs:label>
    <skos:notation rdf:datatype="http://www.w3.org/2001/XMLSchema#string">WP8i</skos:notation>
    <rdfs:range rdf:resource="https://ontology.swissartresearch.net/pwro/WE7_Voyage"/>
  </rdf:Property>
  <rdf:Property rdf:about="https://ontology.swissartresearch.net/pwro/WP9i_was_declared_destination_of">
    <rdfs:domain rdf:resource="http://www.cidoc-crm.org/cidoc-crm/E53_Place"/>
    <rdfs:comment xml:lang="en">This property is the inverse of the forward property described in the scope note that follows. This property links an instance of sending (and its subclasses) with a place of intended destination for the sending of the object. This property links the act of sending with the referenced place through intention, enabling the representation of the intended final arrival spot of the sent object. In documentation, an intended destination may be known rather than an actual destination of arrival for the sent object, or the intended destination and the final destination differ. This property allows the description of this nuance. The property crm:P26_moved_to should be used to document an actual move. For more complex, multi part actions of sending, an event forming part of the overall sending may document the final arrival place of the object (be that at its intended or another location).</rdfs:comment>
    <rdfs:label xml:lang="en">was declared destination of</rdfs:label>
    <skos:notation rdf:datatype="http://www.w3.org/2001/XMLSchema#string">WP9i</skos:notation>
    <rdfs:range rdf:resource="https://ontology.swissartresearch.net/pwro/WE12_Sending"/>
  </rdf:Property>
  <rdf:Property rdf:about="https://ontology.swissartresearch.net/pwro/WP10i_was_diminished_by">
    <rdfs:domain rdf:resource="http://www.cidoc-crm.org/cidoc-crm/E18_Physical_Thing"/>
    <rdfs:comment xml:lang="en">This property is the inverse of the forward property described in the scope note that follows. This property links an instance of destructive physical modification with an instance of physical thing that was diminished through this activity. This property enables the documentation that an instance of destructive physical modification successfully resulted in the reduction of the physical integrity of the physical thing targeted. It does not enable the quantification of this diminishing effect.</rdfs:comment>
    <rdfs:label xml:lang="en">was diminished by</rdfs:label>
    <skos:notation rdf:datatype="http://www.w3.org/2001/XMLSchema#string">WP10i</skos:notation>
    <rdfs:range rdf:resource="https://ontology.swissartresearch.net/pwro/WE9_Destructive_Physical_Modification"/>
    <rdfs:subPropertyOf rdf:resource="http://www.cidoc-crm.org/cidoc-crm/P12i_was_present_at"/>
  </rdf:Property>
  <rdf:Property rdf:about="https://ontology.swissartresearch.net/pwro/WP11i_was_ameliorated_by">
    <rdfs:domain rdf:resource="http://www.cidoc-crm.org/cidoc-crm/E18_Physical_Thing"/>
    <rdfs:comment xml:lang="en">This property is the inverse of the forward property described in the scope note that follows. This property links an instance of ameliorative physical modification with an instance of physical thing that was ameliorated through this activity. This property enables the documentation that an instance of ameliorative physical modification successfully resulted in the improvement of the physical integrity of the physical thing targeted. It does not enable the quantification of this salutary effect.</rdfs:comment>
    <rdfs:label xml:lang="en">was ameliorated by</rdfs:label>
    <skos:notation rdf:datatype="http://www.w3.org/2001/XMLSchema#string">WP11i</skos:notation>
    <rdfs:range rdf:resource="https://ontology.swissartresearch.net/pwro/WE10_Ameliorative_Physical_Modification"/>
    <rdfs:subPropertyOf rdf:resource="http://www.cidoc-crm.org/cidoc-crm/P12i_was_present_at"/>
  </rdf:Property>
  <rdf:Property rdf:about="https://ontology.swissartresearch.net/pwro/WP12i_was_addressee_of">
    <rdfs:domain rdf:resource="https://ontology.swissartresearch.net/aaao/ZE36_Persons"/>
    <rdfs:comment xml:lang="en">This property is the inverse of the forward property described in the scope note that follows. This property links an instance of correspondence event to an instance of  persons to whom it is addressed. This property enables the documentation in a chain of communication of the intended receiver of a particular act of communicating a message.</rdfs:comment>
    <rdfs:label xml:lang="en">was addressee of</rdfs:label>
    <skos:notation rdf:datatype="http://www.w3.org/2001/XMLSchema#string">WP12i</skos:notation>
    <rdfs:range rdf:resource="https://ontology.swissartresearch.net/pwro/WE11_Correspondence_Event"/>
  </rdf:Property>
  <rdf:Property rdf:about="https://ontology.swissartresearch.net/pwro/WP13i_was_declared_origin_of">
    <rdfs:domain rdf:resource="http://www.cidoc-crm.org/cidoc-crm/E53_Place"/>
    <rdfs:comment xml:lang="en">This property is the inverse of the forward property described in the scope note that follows. This property links an instance of sending (and its subclasses) with a place of intended origin for the sending of the object. This property links the act of sending with the referenced place through intention, enabling the representation of the intended originating location of the sending activity. In documentation, an intended origin destination may be known in distinction to the actual origin destination of the sending, and indeed the intended origin location and the final origin location may actually differ. This property allows the description of this nuance. The property crm:P27_moved_from should be used to document an actual origin location. For more complex, multi part actions of sending, an event forming part of the overall sending may document the final origin place of the sending (be that at its intended or another location).</rdfs:comment>
    <rdfs:label xml:lang="en">was declared origin of</rdfs:label>
    <skos:notation rdf:datatype="http://www.w3.org/2001/XMLSchema#string">WP13i</skos:notation>
    <rdfs:range rdf:resource="https://ontology.swissartresearch.net/pwro/WE12_Sending"/>
  </rdf:Property>
  <rdf:Property rdf:about="https://ontology.swissartresearch.net/pwro/WP14i_was_visited_through">
    <rdfs:domain rdf:resource="http://www.cidoc-crm.org/cidoc-crm/E53_Place"/>
    <rdfs:comment xml:lang="en">This property is the inverse of the forward property described in the scope note that follows. This property enables the documentation of the relation of an instance of visit event to the place visited. The relation holding between the visit event and the place differs from the typical documentation of the place at which an event occurs. The documented of the visit relation indicates the intentional activity of the actors involved to interact with and observe the place visited and the objects / events occurring within this place frame.
 </rdfs:comment>
    <rdfs:label xml:lang="en">was visited through</rdfs:label>
    <skos:notation rdf:datatype="http://www.w3.org/2001/XMLSchema#string">WP14i</skos:notation>
    <rdfs:range rdf:resource="https://ontology.swissartresearch.net/pwro/WE13_Visit"/>
    <rdfs:subPropertyOf rdf:resource="http://www.cidoc-crm.org/cidoc-crm/P7i_witnessed"/>
  </rdf:Property>
  <rdf:Property rdf:about="https://ontology.swissartresearch.net/pwro/WP15i_was_dwelt_in_through">
    <rdfs:domain rdf:resource="http://www.cidoc-crm.org/cidoc-crm/E53_Place"/>
    <rdfs:comment xml:lang="en">This property is the inverse of the forward property described in the scope note that follows. This property enables the documentation of the relation of an instance of dwelling event to the place dwelt in. The relation holding between the dwelling event and the place differs from the typical documentation of the place at which an event occurs. The documentation of the dwelling relation indicates the intentional activity of the actors involved to take up phenomenal residence and interact with the place dwelt in and the objects / events occurring therein as part of their everyday life and life activity.</rdfs:comment>
    <rdfs:label xml:lang="en">was dwelt in through</rdfs:label>
    <skos:notation rdf:datatype="http://www.w3.org/2001/XMLSchema#string">WP15i</skos:notation>
    <rdfs:range rdf:resource="https://ontology.swissartresearch.net/pwro/WE14_Dwelling"/>
    <rdfs:subPropertyOf rdf:resource="http://www.cidoc-crm.org/cidoc-crm/P7i_witnessed"/>
  </rdf:Property>
  <rdf:Property rdf:about="https://ontology.swissartresearch.net/pwro/WP16i_was_combatant_in">
    <rdfs:domain rdf:resource="https://ontology.swissartresearch.net/pwro/WE3_Embodied_Actor"/>
    <rdfs:comment xml:lang="en">This property is the inverse of the forward property described in the scope note that follows. This property links an event of attack to instances of embodied actor who actively took part in the physical act of attacking.</rdfs:comment>
    <rdfs:label xml:lang="en">was combatant in</rdfs:label>
    <skos:notation rdf:datatype="http://www.w3.org/2001/XMLSchema#string">WP16i</skos:notation>
    <rdfs:range rdf:resource="https://ontology.swissartresearch.net/pwro/WE6_Attack"/>
    <rdfs:subPropertyOf rdf:resource="http://www.cidoc-crm.org/cidoc-crm/P12i_was_present_at"/>
    <rdfs:subPropertyOf rdf:resource="http://www.cidoc-crm.org/cidoc-crm/P14i_performed"/>
  </rdf:Property>
</rdf:RDF>
